Add rules

theories/glogic.v
@@ -1,4 +1,5 @@
 Require Import stlc.
+Require Import Lia.
 
 
 (*************************)
@@ -14,11 +15,21 @@ Module GLogic (Ty : TY).
     jd_tm : tm
   }.
 
+  Definition wf_judgement C j :=
+    match j with
+    | Build_judgement c t => has_type (C ++ c) t ty_prp
+    end.
+
   Record sequent : Set := {
     sq_context : context;
     sq_premises : list judgement;
     sq_conclusion : judgement
   }.
+
+  Definition wf_sequent s :=
+    match s with
+    | Build_sequent C l j => wf_judgement C j /\ Forall (wf_judgement C) l
+    end.
 
   Notation "|( sig ; l --> B )|" := (Build_sequent sig l B)
     (sig custom stlc_ty, l custom stlc_ty, B custom stlc_ty).
@@ -69,5 +80,87 @@ Module GLogic (Ty : TY).
         has_type (C ++ c) s ty_prp ->
         is_derivable (Build_sequent C l (c :> t)) ->
         is_derivable (Build_sequent C l (c :> tm_or s t))
+    | rl_impL C c l B t s :
+        is_derivable (Build_sequent C l (c :> s)) ->
+        is_derivable (Build_sequent C (c :> t :: l) B) ->
+        is_derivable (Build_sequent C ((c :> tm_imp s t) :: l) B)
+    | rl_impR C c l t s :
+        is_derivable (Build_sequent C (c :> s :: l) (c :> t)) ->
+        is_derivable (Build_sequent C l (c :> tm_imp s t))
+    | rl_forL C c T l B s :
+        has_type (C ++ c) t T ->
+        is_derivable (Build_sequent C ((c :> $(subst (length (C ++ c)) (map tm_lvl (seq 0 (length (C ++ c))) ++ [t]) s)) :: l) B) ->
+        is_derivable (Build_sequent C (c :> $(tm_for T) $(tm_abs T s) :: l) B)
   .
+
+  Theorem th K : is_derivable K -> wf_sequent K.
+  Proof.
+    intros D. induction D; simpl in *.
+    - split; [assumption|].
+      constructor; [assumption|constructor].
+    - destruct IHD2. split; [assumption|].
+      apply Forall_app. split; [intuition|].
+      now inversion H0.
+    - destruct IHD. split; [assumption|].
+      now inversion H0.
+    - destruct IHD. split; [assumption|].
+      constructor; assumption.
+    - split; [assumption|].
+      repeat constructor.
+    - split; constructor.
+    - destruct IHD. split; [assumption|].
+      inversion H1. subst. constructor; [|assumption].
+      simpl. econstructor; [|eassumption].
+      econstructor; [constructor|assumption].
+    - destruct IHD. split; [assumption|].
+      inversion H1; subst. constructor; [|assumption].
+      simpl. econstructor; [|eassumption].
+      econstructor; [constructor|assumption].
+    - intuition.
+      econstructor; [|eassumption].
+      econstructor; [constructor|assumption].
+    - intuition.
+      inversion H0. inversion H2. subst.
+      constructor; [|assumption].
+      econstructor; [|eassumption].
+      econstructor; [constructor|assumption].
+    - intuition.
+      econstructor; [|eassumption].
+      econstructor; [constructor|assumption].
+    - intuition.
+      econstructor; [|eassumption].
+      econstructor; [constructor|assumption].
+    - intuition.
+      inversion H2. subst.
+      constructor; [|assumption].
+      econstructor; [|eassumption].
+      econstructor; [constructor|assumption].
+    - destruct IHD. inversion H0. subst.
+      intuition.
+      econstructor; [|eassumption].
+      econstructor; [constructor|assumption].
+    - intuition. inversion H1. subst.
+      constructor; [|assumption].
+      econstructor; constructor.
+      eapply has_type_subst2 in H4; try eassumption.
+      + repeat rewrite length_app. simpl. lia.
+      + apply Forall2_app.
+        * remember (C0 ++ c) as L.
+          clear dependent C0. clear H.
+          assert (F : forall n, Forall2 (fun (si : tm) (Si : ty) => <| L |- si : Si |>) (map tm_lvl (seq n (length L))) L); [|apply F].
+          replace L with (rev (rev L));
+            [|apply rev_involutive].
+          remember (rev L) as m. clear dependent L.
+          induction m; [constructor|].
+          intros n. simpl.
+          rewrite length_app. rewrite seq_app. simpl.
+          rewrite map_app. simpl.
+          apply Forall2_app.
+          --
+          replace (length (a :: L)) with (S (length L));
+            [|reflexivity].
+          intros n. simpl. constructor.
+          rewrite seq_S. simpl.
+          simpl. constructor.
+  Qed.
 End GLogic.
